theories/Core/Completeness/ContextCases.v
@@ -1,6 +1,7 @@
 From Coq Require Import Morphisms_Relations.
+
 From Mcltt Require Import Base LibTactics.
-From Mcltt.Core Require Import Evaluation Completeness.LogicalRelation Completeness.UniverseCases.
+From Mcltt.Core.Completeness Require Import LogicalRelation UniverseCases.
 Import Domain_Notations.
 
 Proposition valid_ctx_empty :
