theories/Core/Soundness/FunctionCases.v
@@ -3,28 +3,35 @@ From Coq Require Import Morphisms Morphisms_Prop Morphisms_Relations Relation_De
 From Mcltt Require Import Base LibTactics.
 From Mcltt.Core.Completeness Require Import FundamentalTheorem UniverseCases.
 From Mcltt.Core.Semantic Require Import Realizability.
-From Mcltt.Core.Soundness Require Import ContextCases LogicalRelation Realizability.
+From Mcltt.Core.Soundness Require Import ContextCases LogicalRelation SubstitutionCases SubtypingCases TermStructureCases UniverseCases.
 From Mcltt.Core.Syntactic Require Import Corollaries.
 Import Domain_Notations.
 
-Lemma sub_eq_p_q_sigma_compose_tau_extend : forall {Δ' τ Δ M A i σ Γ}, {{ Δ ⊢s σ : Γ }} -> {{ Δ' ⊢s τ : Δ }} -> {{ Γ ⊢ A : Type@i }} -> {{ Δ' ⊢ M : A[σ][τ] }} -> {{ Δ' ⊢s Wk∘(q σ∘(τ,,M)) ≈ σ∘τ : Γ }}.
+Lemma cons_glu_sub_pred_pi_helper : forall {Γ Sb Γ' σ ρ A a i P El Γ'' τ M c},
+    {{ EG Γ ∈ glu_ctx_env ↘ Sb }} ->
+    {{ Γ' ⊢s σ ® ρ ∈ Sb }} ->
+    {{ Γ ⊢ A : Type@i }} ->
+    {{ ⟦ A ⟧ ρ ↘ a }} ->
+    {{ DG a ∈ glu_univ_elem i ↘ P ↘ El }} ->
+    {{ Γ'' ⊢w τ : Γ' }} ->
+    {{ Γ'' ⊢ M : A[σ][τ] ® c ∈ El }} ->
+    {{ Γ'' ⊢s σ∘τ,,M ® ρ ↦ c ∈ cons_glu_sub_pred i Γ A Sb }}.
 Proof.
   intros.
-  assert {{ Γ, A ⊢s Wk : Γ }} by mauto 4.
-  assert {{ Δ, A[σ] ⊢s q σ : Γ, A }} by mauto 4.
-  assert {{ Δ, A[σ] ⊢s Wk∘q σ ≈ σ∘Wk : Γ }} by mauto 4.
-  assert {{ Δ' ⊢s τ,,M : Δ, A[σ] }} by mauto 4.
-  assert {{ Δ, A[σ] ⊢s Wk : Δ }} by mauto 4.
-  assert {{ Δ' ⊢s Wk∘(τ,,M) ≈ τ : Δ }} by mauto 4.
-  assert {{ Δ' ⊢s Wk∘(q σ∘(τ,,M)) ≈ (Wk∘q σ)∘(τ,,M) : Γ }} by mauto 4.
-  assert {{ Δ' ⊢s Wk∘(q σ∘(τ,,M)) ≈ (σ∘Wk)∘(τ,,M) : Γ }} by mauto 4.
-  assert {{ Δ' ⊢s (σ∘Wk)∘(τ,,M) ≈ σ∘(Wk∘(τ,,M)) : Γ }} by mauto 4.
-  assert {{ Δ' ⊢s (σ∘Wk)∘(τ,,M) ≈ σ∘τ : Γ }} by mauto 4.
-  mauto 4.
+  assert {{ Γ' ⊢s σ : Γ }} by mauto 2.
+  assert {{ Γ'' ⊢s τ : Γ' }} by mauto 2.
+  assert {{ Γ'' ⊢ M : A[σ][τ] }} by mauto 2 using glu_univ_elem_trm_escape.
+  assert {{ Γ'' ⊢ M : A[σ∘τ] }} by mauto 3.
+  econstructor; mauto 3;
+    assert {{ Γ'' ⊢s Wk∘(σ∘τ,,M) ≈ σ∘τ : Γ }} as -> by mauto 3.
+  - assert {{ Γ'' ⊢ #0[σ∘τ,,M] ≈ M : A[σ∘τ] }} as -> by mauto 3.
+    assert {{ Γ'' ⊢ A[σ∘τ] ≈ A[σ][τ] : Type@i }} as -> by mauto 3.
+    eassumption.
+  - eapply glu_ctx_env_sub_monotone; mauto 3.
 Qed.
 
-#[export]
-Hint Resolve sub_eq_p_q_sigma_compose_tau_extend : mcltt.
+#[local]
+Hint Resolve cons_glu_sub_pred_pi_helper : mcltt.
 
 Lemma glu_rel_exp_pi : forall {Γ A B i},
     {{ Γ ⊩ A : Type@i }} ->
@@ -34,162 +41,293 @@ Proof.
   intros * HA HB.
   assert {{ Γ ⊢ A : Type@i }} by mauto.
   assert {{ Γ, A ⊢ B : Type@i }} by mauto.
-  assert {{ Γ, A ⊨ B : Type@i }} as HBcomp by mauto using completeness_fundamental_exp.
-  pose proof HA as [SbΓ].
-  pose proof HB as [SbΓA].
-  destruct_conjs.
-  match_by_head glu_ctx_env progressive_invert. (* TODO: define a better inversion tactic for glu_ctx_env *)
-  handle_functional_glu_ctx_env.
-  rename i0 into j.
-  assert {{ EG Γ, A ∈ glu_ctx_env ↘ cons_glu_sub_pred j Γ A TSb }} by (econstructor; try solve_refl; apply_predicate_equivalence; eassumption).
-  destruct (invert_glu_rel_exp ltac:(eassumption) HB) as [k].
-  eexists; split; mauto.
-  eexists (S (max i j)).
+  assert {{ ⊩ Γ }} as [SbΓ] by mauto.
+  assert {{ Γ ⊩ Type@i : Type@(S i) }} by mauto.
+  invert_glu_rel_exp HA.
+  assert {{ EG Γ, A ∈ glu_ctx_env ↘ cons_glu_sub_pred i Γ A SbΓ }} by (econstructor; mauto; reflexivity).
+  assert {{ Γ, A ⊩ Type@i : Type@(S i) }} by mauto.
+  invert_glu_rel_exp HB.
+  eapply glu_rel_exp_of_typ; mauto 3.
   intros.
   assert {{ Δ ⊢s σ : Γ }} by mauto 4.
-  repeat match goal with
-         | H: context[glu_rel_exp_sub _ _ _ _ _ _] |- _ =>
-             match type of H with
-             | __mark__ _ _ => fail 1
-             | _ => edestruct H; [eassumption |]; mark H
-             end
-         end; unmark_all.
+  split; mauto 3.
+  destruct_glu_rel_exp_with_sub.
   simplify_evals.
   match_by_head glu_univ_elem ltac:(fun H => directed invert_glu_univ_elem H).
   handle_functional_glu_univ_elem.
   unfold univ_glu_exp_pred' in *.
   destruct_conjs.
   rename m into a.
-  assert {{ Dom a ≈ a ∈ per_univ i }} as [in_rel] by mauto.
-  assert {{ DG 𝕌@i ∈ glu_univ_elem (S (max i j)) ↘ univ_glu_typ_pred i (S (Nat.max i j)) ↘ univ_glu_exp_pred i (S (Nat.max i j)) }} by (glu_univ_elem_econstructor; lia + reflexivity).
-  pose proof (rel_exp_of_typ_inversion HBcomp) as [env_relΓA].
+  assert {{ Γ ⊨ Π A B : Type@i }} as [env_relΓ]%rel_exp_of_typ_inversion by mauto using completeness_fundamental_exp.
+  assert {{ Γ, A ⊨ B : Type@i }} as [env_relΓA]%rel_exp_of_typ_inversion by mauto using completeness_fundamental_exp.
   destruct_conjs.
+  match_by_head1 (per_ctx_env env_relΓA) invert_per_ctx_env.
   pose env_relΓA.
-  match_by_head (per_ctx_env env_relΓA) invert_per_ctx_env.
-  assert {{ Dom ρ ≈ ρ ∈ tail_rel }} by (eapply glu_ctx_env_per_env; revgoals; eassumption).
-  pose in_rel.
-  destruct_rel_typ.
+  assert {{ Dom ρ ≈ ρ ∈ env_relΓ }} by (eapply glu_ctx_env_per_env; revgoals; eassumption).
+  (on_all_hyp: destruct_rel_by_assumption env_relΓ).
+  simplify_evals.
+  eexists; repeat split; mauto.
+  intros.
+  match_by_head1 glu_univ_elem ltac:(fun H => directed invert_glu_univ_elem H).
   handle_per_univ_elem_irrel.
-  econstructor; mauto.
-  assert (i < S (max i j)) by lia.
-  simpl; repeat split; mauto 3.
-  do 2 eexists.
-  split.
-  - glu_univ_elem_econstructor; mauto; try reflexivity.
-    + instantiate (1 := fun c _ Γ A M m => forall b OPc OElc,
-                            {{ ⟦ B ⟧ ρ ↦ c ↘ b }} ->
-                            {{ DG b ∈ glu_univ_elem i ↘ OPc ↘ OElc }} ->
-                            {{ Γ ⊢ M : A ® m ∈ OElc }}).
-      instantiate (1 := fun c _ Γ A => forall b OPc OElc,
-                            {{ ⟦ B ⟧ ρ ↦ c ↘ b }} ->
-                            {{ DG b ∈ glu_univ_elem i ↘ OPc ↘ OElc }} ->
-                            {{ Γ ⊢ A ® OPc }}).
-      intros.
-      assert {{ Dom ρ ↦ c ≈ ρ ↦ c ∈ env_relΓA }} as HrelΓA by (apply_relation_equivalence; unshelve eexists; mauto 4).
-      apply_relation_equivalence.
-      (on_all_hyp: fun H => destruct (H _ _ HrelΓA)).
-      functional_eval_rewrite_clear.
-      assert (exists P El, {{ DG b ∈ glu_univ_elem i ↘ P ↘ El }}) as [Pb [Elb]] by mauto.
-      eapply simple_glu_univ_elem_morphism_iff; try reflexivity; mauto 3;
-        split; intros; intuition; handle_functional_glu_univ_elem; eassumption.
-    + per_univ_elem_econstructor; mauto; try solve_refl.
-      instantiate (1 := fun c c' _ m m' => forall b b' out_rel,
-                            {{ ⟦ B ⟧ ρ ↦ c ↘ b }} ->
-                            {{ ⟦ B ⟧ ρ ↦ c' ↘ b' }} ->
-                            {{ DF b ≈ b' ∈ per_univ_elem i ↘ out_rel }} ->
-                            {{ Dom m ≈ m' ∈ out_rel }}).
-      intros.
-      assert {{ Dom ρ ↦ c ≈ ρ ↦ c' ∈ env_relΓA }} as HrelΓA by (apply_relation_equivalence; unshelve eexists; mauto 4).
-      apply_relation_equivalence.
-      (on_all_hyp: fun H => destruct (H _ _ HrelΓA)).
-      destruct_by_head per_univ.
-      econstructor; mauto.
-      rewrite <- per_univ_elem_morphism_iff; try reflexivity; mauto.
-      split; intros; intuition; handle_per_univ_elem_irrel; eassumption.
-  - econstructor; mauto 3; intros;
-      assert {{ Δ0 ⊢s σ0 : Δ }} by mauto 2.
-    + assert {{ Δ0 ⊢s σ ∘ σ0 ® ρ ∈ SbΓ }} by (eapply glu_ctx_env_sub_monotone; eassumption).
-      assert (glu_rel_exp_sub H4 Δ0 A {{{ Type @ i }}} {{{ σ ∘ σ0 }}} ρ) as [] by mauto.
-      simplify_evals.
-      match_by_head glu_univ_elem ltac:(fun H => directed invert_glu_univ_elem H).
-      apply_predicate_equivalence.
-      unfold univ_glu_exp_pred' in *.
-      destruct_conjs.
-      handle_functional_glu_univ_elem.
-      enough {{ Δ0 ⊢ A[σ∘σ0] ≈ A[σ][σ0] : Type@i }} as <-; mauto 3.
-    + rename a0 into c.
-      assert {{ Dom ρ ↦ c ≈ ρ ↦ c ∈ env_relΓA }} as HrelΓA by (apply_relation_equivalence; unshelve eexists; mauto 4).
-      apply_relation_equivalence.
-      (on_all_hyp: fun H => destruct (H _ _ HrelΓA)).
-      destruct_by_head per_univ.
-      functional_eval_rewrite_clear.
-      assert {{ Δ, A[σ] ⊢s q σ : Γ, A }} by mauto 3.
-      assert {{ Δ0 ⊢ m : A[σ][σ0] }} by mauto 3 using glu_univ_elem_trm_escape.
-      assert {{ Δ0 ⊢s σ0,,m : Δ, A[σ] }} by mauto 3.
-      repeat match goal with
-             | H: context[glu_rel_typ_sub _ _ _ _ _] |- _ =>
-                 match type of H with
-                 | __mark__ _ _ => fail 1
-                 | _ => edestruct H; [rewrite_predicate_equivalence_left; eassumption |]; mark H
-                 end
-             end; unmark_all.
-      functional_eval_rewrite_clear.
-      assert (cons_glu_sub_pred j Γ A TSb Δ0 {{{ q σ∘(σ0,,m) }}} d{{{ ρ ↦ c }}}) as Hconspred.
-      {
-        assert {{ ⊢ Γ, A }} by mauto 3.
-        assert {{ Γ, A ⊢s Wk : Γ }} by mauto 3.
-        assert {{ Δ0 ⊢s q σ ∘ (σ0,,m) : Γ, A }} by mauto 3.
-        assert {{ Δ0 ⊢s Wk ∘ (q σ ∘ (σ0,,m)) : Γ }} by mauto 3.
-        assert {{ Δ0 ⊢ m : A[σ∘σ0] }} by mauto 3.
-        assert {{ Δ0 ⊢ m : A[σ][σ0] }} by mauto 3.
-        assert {{ Δ0 ⊢s (σ∘σ0),,m : Γ, A }} by mauto 3.
-        assert {{ Δ0 ⊢s q σ ∘ (σ0,,m) ≈ (σ∘σ0),,m : Γ, A }} by mauto 3 using sub_decompose_q.
-        assert {{ Δ0 ⊢ #0[q σ ∘ (σ0,,m)] ≈ #0[(σ∘σ0),,m] : A[Wk][(q σ ∘ (σ0,,m))] }} by mauto 3.
-        econstructor; mauto 3.
-        - assert {{ Δ0 ⊢ #0[q σ ∘ (σ0,,m)] ≈ #0[(σ∘σ0),,m] : A[Wk∘(q σ ∘ (σ0,,m))] }} as -> by mauto 3.
-          assert {{ Δ0 ⊢ #0[(σ∘σ0),,m] ≈ m : A[σ∘σ0] }} by mauto 3.
-          assert {{ Δ0 ⊢s Wk∘(q σ ∘ (σ0,,m)) ≈ σ∘σ0 : Γ }} by mauto 3.
-          assert {{ Δ0 ⊢ #0[(σ∘σ0),,m] ≈ m : A[Wk∘(q σ ∘ (σ0,,m))] }} as -> by mauto 4.
-          assert {{ Δ0 ⊢ A[Wk∘(q σ ∘ (σ0,,m))] ≈ A[σ∘σ0] : Type@j }} as -> by mauto 3.
-          assert {{ Δ0 ⊢ A[σ∘σ0] ≈ A[σ][σ0] : Type@j }} as -> by mauto 3.
-          eapply glu_univ_elem_exp_conv; revgoals; mauto.
-          eapply glu_univ_elem_typ_monotone; mauto.
-        - assert {{ EG Γ ∈ glu_ctx_env ↘ TSb }} by (apply_predicate_equivalence; eassumption).
-          assert {{ Δ0 ⊢s Wk∘(q σ ∘ (σ0,,m)) ≈ σ∘σ0 : Γ }} as -> by mauto 3.
-          eapply glu_ctx_env_sub_monotone; intuition.
-      }
-      (on_all_hyp: fun H => destruct (H _ _ _ Hconspred)).
-      simplify_evals.
-      match_by_head glu_univ_elem ltac:(fun H => directed invert_glu_univ_elem H).
-      apply_predicate_equivalence.
-      unfold univ_glu_exp_pred' in *.
-      destruct_conjs.
-      handle_functional_glu_univ_elem.
-      enough {{ Δ0 ⊢ B[q σ∘(σ0,,m)] ≈ B[q σ][σ0,,m] : Type@i }} as <- by eassumption.
-      assert {{ Δ, A[σ] ⊢s q σ : Γ, A }} by mauto 4.
-      assert {{ Δ0 ⊢ m : A[σ][σ0] }} by mauto 4 using glu_univ_elem_trm_escape.
-      mauto.
+  handle_functional_glu_univ_elem.
+  econstructor; mauto 3; intros Δ' τ **;
+    assert {{ Δ' ⊢s τ : Δ }} by mauto 2.
+  - assert {{ Δ' ⊢s σ ∘ τ ® ρ ∈ SbΓ }} by (eapply glu_ctx_env_sub_monotone; eassumption).
+    assert (glu_rel_exp_with_sub (S i) Δ' A {{{ Type @ i }}} {{{ σ ∘ τ }}} ρ) as [] by mauto.
+    simplify_evals.
+    match_by_head glu_univ_elem ltac:(fun H => directed invert_glu_univ_elem H).
+    apply_predicate_equivalence.
+    unfold univ_glu_exp_pred' in *.
+    destruct_conjs.
+    handle_functional_glu_univ_elem.
+    autorewrite with mcltt.
+    mauto 3.
+  - rename a0 into c.
+    rename equiv_a into equiv_c.
+    assert {{ Dom ρ ↦ c ≈ ρ ↦ c ∈ env_relΓA }} as HrelΓA by (apply_relation_equivalence; unshelve eexists; mauto 4).
+    apply_relation_equivalence.
+    (on_all_hyp: fun H => destruct (H _ _ HrelΓA)).
+    destruct_by_head per_univ.
+    functional_eval_rewrite_clear.
+    rename m0 into b.
+    assert {{ Δ' ⊢ m : A[σ][τ] }} by mauto 3 using glu_univ_elem_trm_escape.
+    assert {{ DG b ∈ glu_univ_elem i ↘ OP c equiv_c ↘ OEl c equiv_c }} by mauto 2.
+    assert {{ Δ' ⊢ B[(σ∘τ),,m] ≈ B[q σ][τ,,m] : Type@i }} as <- by mauto 2 using sub_decompose_q_typ.
+    assert {{ Δ' ⊢s (σ∘τ),,m ® ρ ↦ c ∈ cons_glu_sub_pred i Γ A SbΓ }} as Hconspred by mauto 2.
+    (on_all_hyp: fun H => destruct (H _ _ _ Hconspred)).
+    simplify_evals.
+    match_by_head glu_univ_elem ltac:(fun H => directed invert_glu_univ_elem H).
+    apply_predicate_equivalence.
+    unfold univ_glu_exp_pred' in *.
+    destruct_conjs.
+    handle_functional_glu_univ_elem.
+    eassumption.
 Qed.
 
 #[export]
 Hint Resolve glu_rel_exp_pi : mcltt.
 
-Lemma glu_rel_exp_fn : forall {Γ M A B i},
-    {{ Γ ⊩ A : Type@i }} ->
+Lemma glu_rel_exp_of_pi : forall {Γ M A B i Sb},
+    {{ EG Γ ∈ glu_ctx_env ↘ Sb }} ->
+    {{ Γ ⊨ Π A B : Type@i }} ->
+    (forall Δ σ ρ,
+        {{ Δ ⊢s σ ® ρ ∈ Sb }} ->
+        exists a m,
+          {{ ⟦ A ⟧ ρ ↘ a }} /\
+            {{ ⟦ M ⟧ ρ ↘ m }} /\
+            forall (P : glu_typ_pred) (El : glu_exp_pred), {{ DG Π a ρ B ∈ glu_univ_elem i ↘ P ↘ El }} -> {{ Δ ⊢ M[σ] : (Π A B)[σ] ® m ∈ El }}) ->
+    {{ Γ ⊩ M : Π A B }}.
+Proof.
+  intros * ? [env_relΓ] Hbody.
+  destruct_conjs.
+  eexists; split; mauto.
+  eexists; intros.
+  edestruct Hbody as [? [? [? []]]]; mauto.
+  assert {{ Dom ρ ≈ ρ ∈ env_relΓ }} by (eapply glu_ctx_env_per_env; revgoals; eassumption).
+  (on_all_hyp: destruct_rel_by_assumption env_relΓ).
+  destruct_by_head rel_typ.
+  invert_rel_typ_body.
+  destruct_by_head rel_exp.
+  destruct_conjs.
+  simplify_evals.
+  eapply mk_glu_rel_exp_with_sub''; mauto.
+Qed.
+
+Lemma glu_rel_exp_fn : forall {Γ M A B},
     {{ Γ, A ⊩ M : B }} ->
     {{ Γ ⊩ λ A M : Π A B }}.
-Admitted.
+Proof.
+  intros * HM.
+  assert {{ Γ, A ⊢ M : B }} by mauto 3.
+  assert {{ ⊩ Γ, A }} as [SbΓA] by mauto 3.
+  assert (exists i, {{ Γ, A ⊩ B : Type@i }}) as [i] by mauto 3.
+  invert_glu_rel_exp HM.
+  destruct_conjs.
+  match_by_head (glu_ctx_env SbΓA) invert_glu_ctx_env.
+  rename TSb into SbΓ.
+  rename i0 into j.
+  assert {{ Γ, A ⊢ B : Type@i }} by mauto.
+  assert {{ Γ, A ⊨ M : B }} as [env_relΓA] by mauto using completeness_fundamental_exp.
+  destruct_conjs.
+  pose env_relΓA.
+  match_by_head (per_ctx_env env_relΓA) invert_per_ctx_env.
+  rename tail_rel into env_relΓ.
+  apply_relation_equivalence.
+  assert {{ Γ ⊨ Π A B : Type@(max j i) }} by (mauto using completeness_fundamental_exp).
+  eapply glu_rel_exp_of_pi; mauto.
+  intros.
+  assert {{ Δ ⊢s σ : Γ }} by mauto 4.
+  assert {{ Dom ρ ≈ ρ ∈ env_relΓ }} by (eapply glu_ctx_env_per_env; revgoals; eassumption).
+  destruct_rel_typ.
+  destruct_glu_rel_typ_with_sub.
+  handle_per_univ_elem_irrel.
+  do 2 eexists; repeat split; mauto.
+  intros.
+  match_by_head1 glu_univ_elem ltac:(fun H => directed invert_glu_univ_elem H).
+  handle_per_univ_elem_irrel.
+  apply_predicate_equivalence.
+  match_by_head1 per_univ_elem ltac:(fun H => directed invert_per_univ_elem H).
+  apply_relation_equivalence.
+  assert {{ Δ, A[σ] ⊢ B[q σ] : Type@i }} by mauto 4.
+  econstructor; mauto 4 using lift_exp_max_left, lift_exp_max_right.
+  - intros.
+    assert {{ Dom ρ ↦ c ≈ ρ ↦ c' ∈ env_relΓA }} as HrelΓA by (apply_relation_equivalence; unshelve eexists; mauto 4).
+    destruct_rel_mod_eval.
+    apply_relation_equivalence.
+    (on_all_hyp: fun H => destruct (H _ _ HrelΓA) as [? [[] []]]).
+    handle_per_univ_elem_irrel.
+    econstructor; mauto.
+  - intros.
+    eapply glu_univ_elem_typ_monotone; mauto.
+    eapply glu_univ_elem_typ_cumu_max_left; revgoals; mauto 4.
+  - intros.
+    rename b into c.
+    rename equiv_b into equiv_c.
+    assert {{ Dom ρ ↦ c ≈ ρ ↦ c ∈ env_relΓA }} as HrelΓA by (apply_relation_equivalence; unshelve eexists; mauto 4).
+    destruct_rel_mod_eval.
+    apply_relation_equivalence.
+    (on_all_hyp: fun H => destruct (H _ _ HrelΓA) as [? [[] []]]).
+    handle_per_univ_elem_irrel.
+    eexists; split; mauto.
+    rename a0 into b.
+    assert {{ DG b ∈ glu_univ_elem (max j i) ↘ OP c equiv_c ↘ OEl c equiv_c }} by mauto.
+    assert {{ Δ0 ⊢s σ0 : Δ }} by mauto 3.
+    assert {{ Δ0 ⊢ m' : A[σ][σ0] }} by mauto 3 using glu_univ_elem_trm_escape.
+    assert {{ Δ0 ⊢ m' : A[σ∘σ0] }} by mauto 3.
+    assert {{ Γ, A ⊢ B : Type@(max j i) }} by mauto 2 using lift_exp_max_right.
+    assert {{ Δ0 ⊢ B[(σ∘σ0),,m'] ≈ B[q σ][(σ0,,m')] : Type@(max j i) }} as <- by mauto 2 using sub_decompose_q_typ.
+    assert {{ Δ0 ⊢ (λ A M)[σ][σ0] m' ≈ M[(σ∘σ0),,m'] : B[σ∘σ0,,m'] }} as ->.
+    {
+      assert {{ Δ0 ⊢s σ∘σ0 : Γ }} by mauto 3.
+      assert {{ Γ ⊢ A : Type@(max j i) }} by mauto 2 using lift_exp_max_left.
+      assert {{ Δ0, A[σ∘σ0] ⊢ M[q (σ∘σ0)] : B[q (σ∘σ0)] }} by mauto 3.
+      assert {{ Δ0 ⊢ (λ A M)[σ][σ0] ≈ (λ A M)[σ∘σ0] : (Π A B)[σ∘σ0] }} by (symmetry; mauto 3).
+      assert {{ Δ0 ⊢ (λ A M)[σ][σ0] ≈ (λ A[σ∘σ0] M[q (σ∘σ0)]) : (Π A B)[σ∘σ0] }} by mauto 3.
+      assert {{ Δ0 ⊢ (λ A M)[σ][σ0] ≈ (λ A[σ∘σ0] M[q (σ∘σ0)]) : Π A[σ∘σ0] B[q (σ∘σ0)] }} by mauto 3.
+      assert {{ Δ0 ⊢ (λ A M)[σ][σ0] m' ≈ (λ A[σ∘σ0] M[q (σ∘σ0)]) m' : B[q (σ∘σ0)][Id,,m'] }} by mauto 3.
+      assert {{ Δ0 ⊢ (λ A M)[σ][σ0] m' ≈ M[q (σ∘σ0)][Id,,m'] : B[q (σ∘σ0)][Id,,m'] }} by mauto 3.
+      assert {{ Δ0 ⊢s Id,,m' : Δ0, A[σ∘σ0] }} by mauto 3.
+      assert {{ Δ0, A[σ∘σ0] ⊢s q (σ∘σ0) : Γ, A }} by mauto 2.
+      assert {{ Δ0 ⊢s q (σ∘σ0)∘(Id,,m') : Γ, A }} by mauto 2.
+      assert {{ Δ0 ⊢s q (σ∘σ0)∘(Id,,m') ≈ σ∘σ0,,m' : Γ, A }} by mauto 2.
+      assert {{ Δ0 ⊢ B[q (σ∘σ0)∘(Id,,m')] ≈ B[σ∘σ0,,m'] : Type@i }} as <- by mauto 2.
+      assert {{ Δ0 ⊢ (λ A M)[σ][σ0] m' ≈ M[q (σ∘σ0)][Id,,m'] : B[q (σ∘σ0)∘(Id,,m')] }} as -> by mauto 3.
+      assert {{ Δ0 ⊢ M[q (σ∘σ0)][Id,,m'] ≈ M[q (σ∘σ0)∘(Id,,m')] : B[q (σ∘σ0)∘(Id,,m')] }} as -> by mauto 3.
+      mauto 3.
+    }
+    assert {{ Δ0 ⊢ m' : A[σ][σ0] ® c ∈ El }}
+      by (eapply glu_univ_elem_exp_lower_max_left; mauto 2; eapply glu_univ_elem_typ_monotone; mauto).
+    assert {{ Δ0 ⊢s (σ∘σ0),,m' ® ρ ↦ c ∈ SbΓA }} as HSbΓA by (apply_predicate_equivalence; mauto 2).
+    (on_all_hyp: fun H => destruct (H _ _ _ HSbΓA)).
+    simplify_evals.
+    match_by_head glu_univ_elem ltac:(fun H => directed invert_glu_univ_elem H).
+    eapply glu_univ_elem_exp_cumu_max_right; mauto.
+Qed.
 
 #[export]
 Hint Resolve glu_rel_exp_fn : mcltt.
 
 Lemma glu_rel_exp_app : forall {Γ M N A B i},
-    {{ Γ ⊩ A : Type@i }} ->
     {{ Γ, A ⊩ B : Type@i }} ->
     {{ Γ ⊩ M : Π A B }} ->
     {{ Γ ⊩ N : A }} ->
     {{ Γ ⊩ M N : B[Id,,N] }}.
-Admitted.
+Proof.
+  intros * HB HM HN.
+  assert {{ ⊩ Γ, A }} as [SbΓA] by mauto 3.
+  match_by_head (glu_ctx_env SbΓA) invert_glu_ctx_env.
+  apply_predicate_equivalence.
+  rename i0 into j.
+  rename TSb into SbΓ.
+  assert {{ Γ, A ⊩ Type@i : Type@(S i) }} by mauto 3.
+  assert {{ Γ, A ⊩ B : Type@i }} by mauto 4.
+  invert_glu_rel_exp HB.
+  destruct_conjs.
+  assert {{ Γ ⊩ A : Type@j }} by (eexists; intuition; eexists; mauto 4).
+  assert {{ Γ ⊩ Type@(max i j) : Type@(S (max i j)) }} by mauto 3.
+  assert {{ Γ, A ⊩ Type@(max i j) : Type@(S (max i j)) }} by mauto 3.
+  assert (j <= max i j) by lia.
+  assert {{ Γ ⊩ A : Type@(max i j) }} by mauto 4.
+  assert (i <= max i j) by lia.
+  assert {{ Γ, A ⊩ B : Type@(max i j) }} by mauto 4.
+  assert {{ Γ ⊩ Π A B : Type@(max i j) }} by mauto 3.
+  assert {{ Γ, A ⊢ B : Type@(max i j) }} by mauto 2.
+  assert {{ Γ ⊢ M : Π A B }} by mauto 3.
+  assert {{ Γ ⊢ N : A }} by mauto 3.
+  invert_glu_rel_exp HM.
+  invert_glu_rel_exp HN.
+  eexists; split; [eassumption |].
+  eexists.
+  intros.
+  destruct_glu_rel_typ_with_sub.
+  destruct_glu_rel_exp_with_sub.
+  simplify_evals.
+  rename m into n.
+  rename m0 into m.
+  match_by_head glu_univ_elem ltac:(fun H => directed invert_glu_univ_elem H).
+  handle_functional_glu_univ_elem.
+  match_by_head per_univ_elem ltac:(fun H => directed invert_per_univ_elem H).
+  inversion_clear_by_head pi_glu_exp_pred.
+  assert {{ Dom a ≈ a ∈ per_univ (max i j) }} as [] by mauto.
+  handle_per_univ_elem_irrel.
+  assert {{ Dom n ≈ n ∈ in_rel }} by (eapply glu_univ_elem_per_elem; revgoals; eassumption).
+  (on_all_hyp: destruct_rel_by_assumption in_rel).
+  simplify_evals.
+  rename a0 into b.
+  rename fa into mn.
+  eapply mk_glu_rel_exp_with_sub''; mauto using per_univ_elem_cumu_max_right.
+  intros.
+  match_by_head1 (in_rel n n) ltac:(fun H => rename H into equiv_n).
+  assert {{ DG b ∈ glu_univ_elem (max i j) ↘ OP n equiv_n ↘ OEl n equiv_n }} by mauto 3.
+  assert {{ Δ ⊢ A[σ] ® P0 }} by (eapply glu_univ_elem_trm_typ; eassumption).
+  assert {{ Δ ⊢w Id : Δ }} by mauto 3.
+  assert {{ Δ ⊢ IT[Id] ® P0 }} by mauto 2.
+  assert {{ Δ ⊢ IT[Id] : Type@(max i j) }} by (eapply glu_univ_elem_univ_lvl; revgoals; eassumption).
+  assert {{ Δ ⊢ IT : Type@(max i j) }} by mauto 2.
+  assert {{ Δ ⊢ IT[Id] ≈ A[σ] : Type@(max i j) }} as HAeq by (eapply glu_univ_elem_typ_unique_upto_exp_eq'; revgoals; eassumption).
+  assert {{ Δ ⊢ N[σ] : IT[Id] ® n ∈ El0 }} by (rewrite HAeq; eassumption).
+  assert (exists mn : domain, {{ $| m & n |↘ mn }} /\ {{ Δ ⊢ M[σ][Id] N[σ] : OT[Id,,N[σ]] ® mn ∈ OEl n equiv_n }}) as [] by mauto 2.
+  destruct_conjs.
+  functional_eval_rewrite_clear.
+  assert {{ Δ ⊢ N[σ] : A[σ][Id] ® n ∈ El }}
+    by (autorewrite with mcltt; eapply glu_univ_elem_exp_conv; [| | eassumption | eassumption |]; mauto 3).
+  assert {{ Δ ⊢s σ∘Id,,N[σ] ® ρ ↦ n ∈ cons_glu_sub_pred j Γ A SbΓ }} as Hcons by (apply_predicate_equivalence; mauto 2).
+  (on_all_hyp: destruct_glu_rel_by_assumption (cons_glu_sub_pred j Γ A SbΓ)).
+  simplify_evals.
+  match_by_head glu_univ_elem ltac:(fun H => directed invert_glu_univ_elem H).
+  apply_predicate_equivalence.
+  unfold univ_glu_exp_pred' in *.
+  destruct_conjs.
+  handle_functional_glu_univ_elem.
+  assert {{ Δ ⊢s σ : Γ }} by mauto 2.
+  assert {{ Δ, A[σ] ⊢s q σ : Γ, A }} by mauto 2.
+  assert {{ Γ ⊢s Id,,N : Γ, A }} by mauto 2.
+  assert {{ Δ ⊢ N[σ] : A[σ] }} by mauto 3.
+  assert {{ Δ ⊢s Id,,N[σ] : Δ, A[σ] }} by mauto 3.
+  assert {{ Δ ⊢s σ ≈ σ∘Id : Γ }} by mauto 3.
+  assert {{ Δ ⊢s σ,,N[σ] ≈ (σ∘Id),,N[σ] : Γ, A }} by mauto 3.
+  assert {{ Δ ⊢s (Id,,N)∘σ ≈ σ,,N[σ] : Γ, A }} by mauto 2.
+  autorewrite with mcltt.
+  assert {{ Δ ⊢ B[(Id,,N)∘σ] ≈ B[σ,,N[σ]] : Type@(max i j) }} as -> by mauto 3.
+  assert {{ Δ ⊢ (M N)[σ] ≈ M[σ] N[σ] : B[σ,,N[σ]] }} as -> by mauto 3.
+  assert {{ Δ ⊢ M[σ][Id] N[σ] ≈ M[σ] N[σ] : B[σ,,N[σ]] }} as <-.
+  {
+    assert {{ Δ ⊢ M[σ][Id] ≈ M[σ] : (Π A B)[σ] }} by mauto 2.
+    assert {{ Δ ⊢ M[σ][Id] ≈ M[σ] : Π A[σ] B[q σ] }} by mauto 3.
+    let H := fresh "H" in
+    assert {{ Δ ⊢ M[σ][Id] N[σ] ≈ M[σ] N[σ] : B[q σ][Id,,N[σ]] }} as H by mauto 3;
+    autorewrite with mcltt in H; mauto 3.
+  }
+  assert {{ Δ ⊢ B[σ,,N[σ]] ≈ B[(σ∘Id),,N[σ]] : Type@(max i j) }} as -> by mauto 3.
+  assert {{ Δ ⊢ B[(σ∘Id),,N[σ]] ≈ OT[Id,,N[σ]] : Type@(max i j) }} as ->.
+  {
+    assert {{ Δ ⊢ OT[Id,,N[σ]] ® OP n equiv_n }} by (eapply glu_univ_elem_trm_typ; eassumption).
+    replace (max i j) with (max i (max i j)) by lia.
+    eapply glu_univ_elem_typ_unique_upto_exp_eq; revgoals; eassumption.
+  }
+  eassumption.
+Qed.
 
 #[export]
 Hint Resolve glu_rel_exp_app : mcltt.
