theories/Core/Soundness/SubtypingCases.v
@@ -13,47 +13,26 @@ Lemma glu_rel_exp_subtyp : forall {Γ M A A' i},
     {{ Γ ⊢ A ⊆ A' }} ->
     {{ Γ ⊩ M : A' }}.
 Proof.
-  intros * [Sb [? [i]]] HA' [env_relΓ [? [j]]]%completeness_fundamental_subtyp.
+  intros * [] HA' [env_relΓ [? [k]]]%completeness_fundamental_subtyp.
   destruct_conjs.
-  eapply invert_glu_rel_exp in HA'; try eassumption.
-  destruct_conjs.
-  rename i0 into k.
+  invert_glu_rel_exp HA'.
   econstructor; split; [eassumption |].
-  exists (max i (max j k)); intros.
-  (* TODO: extract this as a tactic *)
-  repeat match goal with
-         | H: context[glu_rel_exp_sub _ _ _ _ _ _] |- _ =>
-             match type of H with
-             | __mark__ _ _ => fail 1
-             | _ => edestruct H; try eassumption; mark H
-             end
-         end; unmark_all.
+  exists (max i k); intros.
+  destruct_glu_rel_exp_with_sub.
   simplify_evals.
   match_by_head glu_univ_elem ltac:(fun H => directed invert_glu_univ_elem H).
   handle_functional_glu_univ_elem.
-  rename m into a'.
-  rename a0 into a.
-  rename m0 into m.
-  rename P0 into P.
-  rename El0 into El.
   assert {{ Dom ρ ≈ ρ ∈ env_relΓ }} by (eapply glu_ctx_env_per_env; mauto).
   (on_all_hyp: destruct_rel_by_assumption env_relΓ).
+  destruct_by_head rel_typ.
   destruct_by_head rel_exp.
   handle_per_univ_elem_irrel.
   unfold univ_glu_exp_pred' in *.
   destruct_conjs.
-  assert (exists P El, glu_univ_elem (max i (max j k)) P El a') as [? []].
-  {
-    assert (exists P El, glu_univ_elem (max j k) P El a') as [? []];
-      mauto using glu_univ_elem_cumu_max_right.
-  }
-  econstructor; try eassumption.
-  assert {{ Sub a <: a' at max i (max j k) }} by mauto using per_subtyp_cumu_left, per_subtyp_cumu_right.
-  assert (exists P El, glu_univ_elem (max i (max j k)) P El a) as [? []] by mauto using glu_univ_elem_cumu_max_left.
-  eapply glu_univ_elem_per_subtyp_trm_if; mauto.
-  - assert (k <= max i (max j k)) by lia.
-    eapply glu_univ_elem_typ_cumu_ge; revgoals; mauto.
-  - eapply glu_univ_elem_exp_cumu_max_left; revgoals; mauto.
+  eapply mk_glu_rel_exp_with_sub''; gintuition mauto using per_univ_elem_cumu_max_left, per_univ_elem_cumu_max_right.
+  eapply glu_univ_elem_per_subtyp_trm_conv; mauto.
+  assert (i <= max i k) by lia.
+  eapply glu_univ_elem_typ_cumu_ge; revgoals; mauto.
 Qed.
 
 #[export]
@@ -65,21 +44,13 @@ Lemma glu_rel_sub_subtyp : forall {Γ σ Δ Δ'},
     {{ ⊢ Δ ⊆ Δ' }} ->
     {{ Γ ⊩s σ : Δ' }}.
 Proof.
-  intros * [SbΓ [SbΔ]] [SbΔ'] Hsubtyp.
-  pose proof (completeness_fundamental_ctx_subtyp _ _ Hsubtyp).
+  intros * [] [] Hsubtyp.
   destruct_conjs.
   econstructor; eexists; repeat split; [eassumption | eassumption |].
   intros.
-  (* TODO: extract this as a tactic *)
-  repeat match goal with
-         | H: context[glu_rel_sub_sub _ _ _ _ _] |- _ =>
-             match type of H with
-             | __mark__ _ _ => fail 1
-             | _ => edestruct H; try eassumption; mark H
-             end
-         end; unmark_all.
+  destruct_glu_rel_sub_with_sub.
   econstructor; mauto.
-  eapply glu_ctx_env_per_ctx_subtyp_sub_if; mauto.
+  eapply glu_ctx_env_subtyp_sub_if; mauto.
 Qed.
 
 #[export]
