theories/Core/Soundness/UniverseCases.v
@@ -7,19 +7,39 @@ From Mcltt.Core.Soundness Require Import LogicalRelation Realizability.
 From Mcltt.Core.Syntactic Require Import Corollaries.
 Import Domain_Notations.
 
+Lemma glu_rel_exp_of_typ : forall {Γ Sb A i},
+    {{ EG Γ ∈ glu_ctx_env ↘ Sb }} ->
+    (forall Δ σ ρ,
+        {{ Δ ⊢s σ ® ρ ∈ Sb }} ->
+        {{ Δ ⊢ A[σ] : Type@i }} /\
+          exists a,
+            {{ ⟦ A ⟧ ρ ↘ a }} /\
+              {{ Dom a ≈ a ∈ per_univ i }} /\
+              forall P El, {{ DG a ∈ glu_univ_elem i ↘ P ↘ El }} -> {{ Δ ⊢ A[σ] ® P }}) ->
+    {{ Γ ⊩ A : Type@i }}.
+Proof.
+  intros * ? Hbody.
+  eexists; split; mauto.
+  exists (S i).
+  intros.
+  edestruct Hbody as [? [? [? []]]]; mauto.
+Qed.
+
 Lemma glu_rel_exp_typ : forall {Γ i},
     {{ ⊩ Γ }} ->
     {{ Γ ⊩ Type@i : Type@(S i) }}.
 Proof.
-  intros * [Sb].
-  eexists; split; [eassumption |].
-  eexists.
+  intros * [].
+  eapply glu_rel_exp_of_typ; mauto 3.
   intros.
-  econstructor; mauto.
-  repeat split; mauto.
-  do 2 eexists; split; mauto.
-  cbv.
-  mauto.
+  assert {{ Δ ⊢s σ : Γ }} by mauto 3.
+  split; mauto 4.
+  eexists; repeat split; mauto.
+  intros.
+  match_by_head1 glu_univ_elem invert_glu_univ_elem.
+  apply_predicate_equivalence.
+  cbn.
+  mauto 4.
 Qed.
 
 #[export]
